proof/refine/RISCV64/Retype_R.thy
@@ -82,8 +82,9 @@ definition makeObjectKO
     | Inr (APIObjectType ArchTypes_H.CapTableObject) \<Rightarrow> Some (KOCTE makeObject)
     | Inr (APIObjectType ArchTypes_H.ReplyObject) \<Rightarrow> Some (KOReply makeObject)
     | Inr (APIObjectType ArchTypes_H.SchedContextObject) \<Rightarrow>
-                Some (KOSchedContext (scRefills_update
-                   (\<lambda>_. replicate (refillAbsoluteMax' us) emptyRefill) makeObject))
+            Some (KOSchedContext ((makeObject :: sched_context)
+                                     \<lparr>scRefills := replicate (refillAbsoluteMax' us) emptyRefill,
+                                      scSize := us - minSchedContextBits\<rparr>))
     | Inr PageTableObject \<Rightarrow> Some (KOArch (KOPTE makeObject))
     | Inr SmallPageObject \<Rightarrow> Some (if dev then KOUserDataDevice else KOUserData)
     | Inr LargePageObject \<Rightarrow> Some(if dev then KOUserDataDevice else KOUserData)
@@ -129,7 +130,8 @@ lemma valid_obj_makeObject_reply [simp]:
 lemma valid_sc_size'_makeObject_sc':
   "sc_size_bounds us \<Longrightarrow>
      valid_sched_context_size'
-       (scRefills_update (\<lambda>_. replicate (refillAbsoluteMax' us) emptyRefill) makeObject)"
+       ((makeObject :: sched_context)\<lparr>scRefills := replicate (refillAbsoluteMax' us) emptyRefill,
+                                      scSize := us - minSchedContextBits\<rparr>)"
   by (clarsimp simp: makeObject_sc valid_sched_context_size'_def scBits_simps
                      objBits_def objBitsKO_def)
 
@@ -139,12 +141,13 @@ lemma MIN_REFILLS_refillAbsoluteMax'[simp]:
 
 lemma valid_obj_makeObject_sched_context [simp]:
   "sc_size_bounds us \<Longrightarrow>
-     valid_obj' (KOSchedContext (scRefills_update
-                   (\<lambda>_. replicate (refillAbsoluteMax' us) emptyRefill) makeObject)) s"
+     valid_obj' (KOSchedContext ((makeObject :: sched_context)
+                                    \<lparr>scRefills := replicate (refillAbsoluteMax' us) emptyRefill,
+                                     scSize := us - minSchedContextBits\<rparr>)) s"
   unfolding valid_obj'_def valid_sched_context'_def
   using refillAbsoluteMax'_lb sc_size_bounds_def minRefillLength_ARM
   by (clarsimp simp: valid_sc_size'_makeObject_sc')
-     (clarsimp simp: makeObject_sc scBits_inverse_us)
+     (clarsimp simp: makeObject_sc)
 
 lemma valid_obj_makeObject_user_data [simp]:
   "valid_obj' (KOUserData) s"
@@ -844,7 +847,7 @@ lemma objBits_le_obj_bits_api:
    makeObjectKO dev us d ty = Some ko \<Longrightarrow>
    objBitsKO ko \<le> obj_bits_api (APIType_map2 ty) us"
   apply (case_tac ty)
-   by (auto simp: default_arch_object_def pageBits_def archObjSize_def pteBits_def
+   by (auto simp: default_arch_object_def pageBits_def pteBits_def
                   makeObjectKO_def objBits_simps' APIType_map2_def obj_bits_api_def slot_bits_def
                   scBits_simps table_size_def
            split: Structures_H.kernel_object.splits arch_kernel_object.splits object_type.splits
@@ -1574,7 +1577,7 @@ lemma new_cap_addrs_fold':
 
 lemma objBitsKO_gt_0: "0 < objBitsKO ko"
   apply (case_tac ko)
-        apply (simp_all add:objBits_simps' pageBits_def)
+        apply (simp_all add: objBits_simps' bit_simps')
   apply (rename_tac arch_kernel_object)
   apply (case_tac arch_kernel_object)
     apply (simp_all add:archObjSize_def bit_simps)
@@ -2459,8 +2462,9 @@ lemma refillAbsoluteMax'_gt1:
 lemma sc_relation_retype:
   "\<lbrakk>sc_size_bounds n\<rbrakk> \<Longrightarrow>
    obj_relation_retype (default_object Structures_A.SchedContextObject dev n d)
-                         (KOSchedContext (scRefills_update
-                            (\<lambda>_. replicate (refillAbsoluteMax' n) emptyRefill) makeObject))"
+                       (KOSchedContext ((makeObject :: sched_context)
+                                           \<lparr>scRefills := replicate (refillAbsoluteMax' n) emptyRefill,
+                                            scSize := n - minSchedContextBits\<rparr>))"
   by (clarsimp simp: default_object_def sc_relation_def default_sched_context_def
                      makeObject_sc obj_relation_retype_def valid_sched_context_size_def
                      objBits_simps word_bits_def scBits_simps refills_map_def refill_map_def
@@ -4486,12 +4490,12 @@ lemma createNewCaps_valid_pspace:
              apply (rule hoare_assume_pre)
   by (wpsimp wp: createObjects_valid_pspace_untyped'[of dev us _ "Inr ty", where ptr=ptr]
                  mapM_x_wp'
-          split_del: if_split
-          simp: createObjects_def makeObjectKO_def objBits_def objBitsKO_def scBits_simps
-                power_add not_0 APIType_capBits_def field_simps pageBits_def
-                archObjSize_def ptBits_def pteBits_def scBits_simps
-                ptTranslationBits_def pt_bits_def pte_bits_def word_size_bits_def table_size_def
-    | simp)+
+      split_del: if_split
+           simp: createObjects_def makeObjectKO_def objBits_def objBitsKO_def scBits_simps
+                 not_0 APIType_capBits_def field_simps pageBits_def
+                 archObjSize_def ptBits_def pteBits_def scBits_simps
+                 ptTranslationBits_def pt_bits_def pte_bits_def word_size_bits_def table_size_def
+      | simp add: power_add)+
 
 lemma copyGlobalMappings_inv[wp]:
   "\<lbrace>\<lambda>s. P (ksMachineState s)\<rbrace>
